Copy mem automation

new/golang/defn/dynamic_mem.v
@@ -7,12 +7,9 @@ From Perennial Require Import base.
 Section defn.
 Context `{ffi_syntax}.
 
-(* note this takes a type to make it syntactically part of the code, but it is
-not needed at runtime (same as the mem.v version, except that we take the
-type as a GooseLang argument rather than a Gallina argument) *)
-Definition ref_ty_def : val := λ: "t" "v", ref (Var "v").
-Program Definition ref_ty := sealed @ref_ty_def.
-Definition ref_ty_unseal : ref_ty = _ := seal_eq _.
+Definition alloc_def : val := λ: "v", ref (Var "v").
+Program Definition alloc := sealed @alloc_def.
+Definition alloc_unseal : alloc = _ := seal_eq _.
 
 Definition load_ty_def: val :=
   rec: "go" "t" "l" :=
