new/golang/defn.v
@@ -1,4 +1,6 @@
 From Perennial.goose_lang Require Export lang notation.
+(* NOTE: dynamic_mem should replace mem, not used yet *)
+From New.golang.defn Require dynamic_mem.
 From New.golang.defn Require Export exception list typing dynamic_typing noop loop struct mem
   slice map string interface defer chan builtin array globals pkg.
 Open Scope struct_scope.
