new/golang/theory/dynamic_mem.v
@@ -1,5 +1,8 @@
-From Coq Require Import Program.Equality.
+From iris.proofmode Require Import coq_tactics reduction.
+From iris.proofmode Require Import tactics.
+From iris.proofmode Require Import environments.
 From New.golang.theory Require Import proofmode.
+From iris.proofmode Require Import string_ident.
 From Ltac2 Require Import Ltac2.
 Set Default Proof Mode "Classic".
 From New.golang.theory Require Import typing assume list mem dynamic_typing.
@@ -13,13 +16,13 @@ Context `{!IntoVal V}.
 
 Context `{!IntoValTyped V t}.
 
-Lemma wp_ref_ty (v : V) stk E :
+Lemma wp_alloc (v : V) stk E :
   {{{ True }}}
-    ref_ty #t (# v) @ stk; E
+    alloc (# v) @ stk; E
   {{{ l, RET #l; l ↦ v }}}.
 Proof.
   iIntros (Φ) "_ HΦ".
-  rewrite ref_ty_unseal.
+  rewrite alloc_unseal.
   wp_call.
   iApply (wp_alloc1_seq with "[//]"). iNext.
   iIntros (l) "Hl".
@@ -170,3 +173,145 @@ Proof.
 Admitted.
 
 End goose_lang.
+
+Section tac_lemmas.
+  Context `{ffi_sem: ffi_semantics} `{!ffi_interp ffi} `{!heapGS Σ}.
+
+  Lemma tac_wp_load_ty {V t} `{!IntoVal V} `{!IntoValTyped V t}
+    K (l : loc) (v : V) Δ s E i dq Φ is_pers
+    `{!PointsToAccess l v dq P P'} :
+    envs_lookup i Δ = Some (is_pers, P)%I →
+    envs_entails Δ (WP (fill K (Val #v)) @ s; E {{ Φ }}) →
+    envs_entails Δ (WP (fill K (load_ty #t #l)) @ s; E {{ Φ }}).
+  Proof using Type*.
+    rewrite envs_entails_unseal => ? HΦ.
+    rewrite envs_lookup_split //.
+    iIntros "[H Henv]".
+    destruct is_pers; simpl.
+    - iDestruct "H" as "#H".
+      iDestruct (points_to_acc with "H") as "[H' _]".
+      wp_apply (wp_load_ty with "[$]").
+      iIntros "?".
+      iApply HΦ. iApply "Henv". iFrame "#".
+    - iDestruct (points_to_acc with "H") as "[H Hclose]".
+      wp_apply (wp_load_ty with "[$]").
+      iIntros "?".
+      iApply HΦ. iApply "Henv".
+      iSpecialize ("Hclose" with "[$]").
+      rewrite points_to_update_eq. iFrame.
+  Qed.
+
+  Lemma tac_wp_store_ty {V t} `{!IntoVal V} `{!IntoValTyped V t}
+    K (l : loc) (v v' : V) Δ Δ' s E i Φ
+    `{!PointsToAccess l v (DfracOwn 1) P P'} :
+    envs_lookup i Δ = Some (false, P)%I →
+    envs_simple_replace i false (Esnoc Enil i (P' v')) Δ = Some Δ' →
+    envs_entails Δ' (WP fill K (Val #()) @ s ; E {{ Φ }}) →
+    envs_entails Δ (WP (fill K (store_ty #t #l (Val #v'))) @ s; E {{ Φ }}).
+  Proof.
+    rewrite envs_entails_unseal => ?? HΦ.
+    rewrite envs_simple_replace_sound // /=.
+    iIntros "[H Henv]".
+    iDestruct (points_to_acc with "H") as "[H Hclose]".
+    wp_apply (wp_store_ty with "[$]").
+    iIntros "H". iSpecialize ("Hclose" with "[$]").
+    iApply HΦ.
+    iApply "Henv". iFrame.
+  Qed.
+
+  Lemma tac_wp_alloc
+    `{!IntoVal V}
+    K Δ stk E (v : V) Φ :
+    (∀ l, envs_entails Δ (l ↦ v -∗ WP (fill K (Val #l)) @ stk; E {{ Φ }})) →
+    envs_entails Δ (WP fill K (alloc #v) @ stk; E {{ Φ }}).
+  Proof.
+    rewrite envs_entails_unseal => Hwp.
+    iIntros "Henv".
+    wp_apply wp_alloc. iIntros.
+    by iApply (Hwp with "[$]").
+  Qed.
+
+  Global Instance points_to_access_trivial {V} l (v : V) {t} `{!IntoVal V} `{!IntoValTyped V t} dq
+    : PointsToAccess l v dq (l ↦{dq} v)%I (λ v', l ↦{dq} v')%I.
+  Proof. constructor; [eauto with iFrame|done]. Qed.
+
+End tac_lemmas.
+
+Ltac2 wp_load_visit e k :=
+  Control.once_plus (fun () => Std.unify e '(load_ty (Val _) (Val _)))
+         (fun _ => Control.zero Walk_expr_more);
+  Control.once_plus (fun _ => eapply (tac_wp_load_ty $k) > [tc_solve_many ()| ltac1:(iAssumptionCore) | ectx_simpl ()])
+    (fun _ => Control.backtrack_tactic_failure "wp_load: could not find a points-to in context covering the address")
+.
+
+Ltac2 wp_load () :=
+  lazy_match! goal with
+  | [ |- envs_entails _ (wp _ _ ?e _) ] => wp_walk_unwrap (fun () => walk_expr e wp_load_visit)
+                                                        "wp_load: could not find load_ty"
+  | [ |- _ ] => Control.backtrack_tactic_failure "wp_load: not a wp"
+  end.
+
+Ltac2 wp_store_visit e k :=
+  Control.once_plus (fun () => (Std.unify e '(store_ty _ _ (Val _))))
+         (fun _ => Control.zero Walk_expr_more);
+  Control.once_plus (fun _ => eapply (tac_wp_store_ty $k) > [tc_solve_many ()| ltac1:(iAssumptionCore)
+                                           |ltac1:(pm_reflexivity) | ectx_simpl () ])
+    (fun _ => Control.backtrack_tactic_failure "wp_store: could not find a points-to in context covering the address")
+.
+
+Ltac2 wp_store () :=
+  lazy_match! goal with
+  | [ |- envs_entails _ (wp _ _ ?e _) ] => wp_walk_unwrap (fun () => walk_expr e wp_store_visit)
+                                                        "wp_store: could not find store_ty"
+  | [ |- _ ] => Control.backtrack_tactic_failure "wp_store: not a wp"
+  end.
+
+Ltac2 wp_alloc_visit e k :=
+  Control.once_plus (fun () => Std.unify e '(alloc (Val _)))
+    (fun _ => Control.zero Walk_expr_more);
+  Control.once_plus (fun _ => eapply (tac_wp_alloc $k); ectx_simpl ())
+    (fun _ => Control.backtrack_tactic_failure "wp_alloc: failed to apply tac_wp_alloc")
+.
+
+Ltac2 wp_alloc () :=
+  lazy_match! goal with
+  | [ |- envs_entails _ (wp _ _ ?e _) ] => wp_walk_unwrap (fun () => walk_expr e wp_alloc_visit)
+                                                        "wp_alloc: could not find ref_ty"
+  | [ |- _ ] => Control.backtrack_tactic_failure "wp_alloc: not a wp"
+  end.
+
+Ltac2 wp_alloc_auto_visit e k :=
+  lazy_match! e with
+  (* Manually writing out [let: ?var_name := (alloc (Val _)) in ?e1] to get
+     pattern matching to work. *)
+  | (App (Rec BAnon (BNamed ?var_name) ?e1) (App (Val alloc) (Val _))) =>
+      let let_expr1 := '(Rec BAnon (BNamed $var_name) $e1) in
+      let ptr_name := Std.eval_vm None constr:($var_name +:+ "_ptr") in
+      let k := constr:(@AppRCtx _ $let_expr1 :: $k) in
+      Control.once_plus (fun _ => eapply (tac_wp_alloc $k); ectx_simpl ())
+        (fun _ => Control.backtrack_tactic_failure "wp_alloc_auto: failed to apply tac_wp_ref_ty");
+      let i :=
+        orelse (fun () => Option.get_bt (Ident.of_string (StringToIdent.coq_string_to_string ptr_name)))
+          (fun _ => Control.backtrack_tactic_failure "wp_alloc_auto: could not convert to ident") in
+      Std.intros false [Std.IntroNaming (Std.IntroIdentifier i)];
+      ltac1:(hyp_name |- iIntros hyp_name) (Ltac1.of_constr var_name)
+  | _ => Control.zero Walk_expr_more
+  end.
+
+Ltac2 wp_alloc_auto () :=
+  lazy_match! goal with
+  | [ |- envs_entails _ (wp _ _ ?e _) ] => wp_walk_unwrap (fun () => walk_expr e wp_alloc_auto_visit)
+                                                        "wp_alloc_auto: could not find ref_ty"
+  | [ |- _ ] => Control.backtrack_tactic_failure "wp_alloc_auto: not a wp"
+  end.
+
+Tactic Notation "wp_alloc_auto" :=
+  ltac2:(Control.enter wp_alloc_auto).
+
+Tactic Notation "wp_alloc" ident(l) "as" constr(H) :=
+  ltac2:(Control.enter wp_alloc);
+  intros l;
+  iIntros H.
+
+Tactic Notation "wp_load" := ltac2:(Control.enter wp_load).
+Tactic Notation "wp_store" := ltac2:(Control.enter wp_store).
